---
date: 2024-11-04T10:09:06
publish: true
comments: true
permalink: eigenvalue
aliases:
---

# 特征值

$$
y(k) + a_{n-1} y(k-1) + \cdots + a_0 y(k-n) = 0
$$

$$
\begin{bmatrix}
y(k)\\ 
y(k-1)\\
\vdots\\
y(k-n+1)
\end{bmatrix}=\begin{bmatrix}
-a_{n-1} &-a_{n-2} &\cdots  &-a_0 \\
1 & & & \\
&\ddots & & \\
& &1 &
\end{bmatrix}\begin{bmatrix}
y(k-1)\\
y(k-2)\\
\vdots\\
y(k-n)
\end{bmatrix}
$$

$$
\begin{vmatrix}
-a_{n-1}-\lambda &-a_{n-2} &\cdots  &-a_0 \\
1 &-\lambda & & \\
&\ddots &\ddots & \\
& &1 &-\lambda
\end{vmatrix}=0
$$

$$
\begin{vmatrix}
-\lambda - \displaystyle\sum_{i=0}^{n-1} \lambda^{-i}a_{n-1-i} &-\displaystyle\sum_{i=0}^{n-2} \lambda^{-i}a_{n-2-i} &\cdots  &-a_0 \\
 &-\lambda & & \\
& &\ddots & \\
& & &-\lambda
\end{vmatrix}=0
$$

$$
(-\lambda)^{n-1}\left ( -\lambda - \displaystyle\sum_{i=0}^{n-1} \lambda^{-i}a_{n-1-i} \right )=0
$$

$$
\lambda^n + \displaystyle\sum_{i=0}^{n-1} \lambda^{i}a_{i}=0
$$
